PProperties.v
@@ -19,8 +19,9 @@ Proof.
     repeat split; eauto.
     + rewrite <- H2; assumption.
     + econstructor 1; auto.
-      * unfold key_not_In in HDisjCalls.
-        intro; specialize (HDisjCalls v); rewrite H2 in HDisjCalls; eauto.
+      * intro; apply HDisjCalls; rewrite H2; assumption.
+        (* unfold key_not_In in HDisjCalls. *)
+        (* intro; specialize (HDisjCalls v); rewrite H2 in HDisjCalls; eauto. *)
   - exists x, x0, x1.
     repeat split; eauto.
     econstructor 2; assumption.
@@ -29,7 +30,8 @@ Proof.
     repeat split; auto.
     + econstructor 3; eauto.
       * intro; specialize (HDisjRegs k0); rewrite <- H6, <- H2; assumption.
-      * intro; specialize (HDisjCalls k0); rewrite <- H7, <- H3; assumption.
+      * intro; specialize (HDisjCalls x5); rewrite <-H7, <-H3; assumption.
+        (* intro; specialize (HDisjCalls k0); rewrite <- H7, <- H3; assumption. *)
   - exists x, x0, x1.
     repeat split; auto.
     econstructor 4; eauto.
@@ -45,17 +47,17 @@ Proof.
   - exists (x2++x), (x3++x0), (x4++x1).
     rewrite H1, H5 in HUReadRegs; rewrite H2, H6 in HUNewRegs; rewrite H3, H7 in HUCalls.
     repeat split; auto.
-    econstructor 7; auto.
+    econstructor 7 with (calls1 := x4) (calls2 := x1); auto.
     + intro; specialize (HDisjRegs k); rewrite H2, H6 in HDisjRegs; apply HDisjRegs.
-    + intro; specialize (HDisjCalls k); rewrite H3, H7 in HDisjCalls; apply HDisjCalls.
+    + intro; specialize (HDisjCalls x5); rewrite H3, H7 in HDisjCalls; apply HDisjCalls.
     + apply H8.
     + assumption.
   - exists (x2++x), (x3++x0), (x4++x1).
     rewrite H1, H5 in HUReadRegs; rewrite H2, H6 in HUNewRegs; rewrite H3, H7 in HUCalls.
     repeat split; auto.
-    econstructor 8; auto.
+    econstructor 8 with (calls1:=x4)(calls2:=x1); auto.
     + intro; specialize (HDisjRegs k); rewrite H2, H6 in HDisjRegs; apply HDisjRegs.
-    + intro; specialize (HDisjCalls k); rewrite H3, H7 in HDisjCalls; apply HDisjCalls.
+    + intro; specialize (HDisjCalls x5); rewrite H3, H7 in HDisjCalls; apply HDisjCalls.
     + apply H8.
     + assumption.
   - exists x, x0, x1.
